experiments/state_on_io/MIO.Sig.fst
@@ -8,6 +8,7 @@ include Hist
 
 unfold let no_cf (a:Type0) = r:resexn a{~(r == Inr Contract_failure)}
 
+(** IO commands (parameterize the free monad). *)
 noeq
 type io_cmds : Type0 -> Type0 =
 | Openfile : string -> io_cmds (no_cf file_descr)
@@ -17,14 +18,16 @@ type io_cmds : Type0 -> Type0 =
 
 type caller = Free.caller
 
+(** IO events (parameterize the hist monad).
+    Each event records the command, caller, and result. *)
 noeq
-type event =
-  | EOpenfile : caller -> string -> no_cf file_descr -> event
-  | ERead     : caller -> file_descr -> no_cf string -> event
-  | EWrite    : caller -> file_descr -> string -> no_cf unit -> event
-  | EClose    : caller -> file_descr -> no_cf unit -> event
+type io_event =
+  | EOpenfile : caller -> string -> no_cf file_descr -> io_event
+  | ERead     : caller -> file_descr -> no_cf string -> io_event
+  | EWrite    : caller -> file_descr -> string -> no_cf unit -> io_event
+  | EClose    : caller -> file_descr -> no_cf unit -> io_event
 
-type trace = list event
+type trace = list io_event
 
 (** We only need GetTrace/GetST because we assume that our actions are
 updating the trace for us. Therefore, at extraction, our actions
@@ -42,7 +45,7 @@ type mstate = {
 }
 
 type mst_updater (mst:mstate) : Type0 =
-  s0:mst.typ -> e:event -> h : Ghost.erased trace ->
+  s0:mst.typ -> e:io_event -> h : Ghost.erased trace ->
   Pure mst.typ
        (requires mst.abstracts s0 h)
        (ensures fun s1 -> mst.abstracts s1 (e::h))
@@ -53,12 +56,14 @@ type mst_impl (mst:mstate) = {
   update : mst_updater mst;
 }
 
+(** Monitoring commands. *)
 noeq
 type m_cmds (mst:mstate) : Type0 -> Type0 =
 | GetTrace : m_cmds mst (Ghost.erased trace)
 | GetST    : m_cmds mst mst.typ
 
-let mio_cmds (mst:mstate) : Type0 -> Type u#1 = ev_sum io_cmds (m_cmds mst)
+(** Combined MIO commands = io_cmds + m_cmds. *)
+let mio_cmds (mst:mstate) : Type0 -> Type u#1 = cmd_sum io_cmds (m_cmds mst)
 
 // THE MIO FREE MONAD
 type mio (mst:mstate) (a:Type) = free (mio_cmds mst) a
@@ -72,9 +77,9 @@ let mio_bind #mst (#a:Type) (#b:Type) l k : mio mst b =
 let convert_call_to_event
   (c:caller)
   (#r:Type0)
-  (cmd:io_cmds r)
-  (res:r) : event =
-  match cmd with
+  (op:io_cmds r)
+  (res:r) : io_event =
+  match op with
   | Openfile arg -> EOpenfile c arg res
   | Read arg     -> ERead c arg res
   | Write fd s   -> EWrite c fd s res
@@ -85,7 +90,7 @@ unfold
 let apply_changes (history local_events:trace) : Tot trace =
   (List.rev local_events) @ history
 
-let destruct_event (e:event) : (caller & r:Type0 & io_cmds r & r) =
+let destruct_event (e:io_event) : (caller & r:Type0 & io_cmds r & r) =
   match e with
   | EOpenfile c arg res -> (| c, no_cf file_descr, Openfile arg, res |)
   | ERead c arg res     -> (| c, no_cf string, Read arg, res |)
@@ -104,59 +109,60 @@ let rec is_open (fd:file_descr) (h:trace) : bool =
                     else is_open fd tail
                | _ -> is_open fd tail
 
-unfold let io_pre (#r:Type0) (cmd:io_cmds r) (h:trace) : Type0 =
+unfold let io_pre (#r:Type0) (op:io_cmds r) (h:trace) : Type0 =
   True
 
-unfold let io_post (#r:Type0) (cmd:io_cmds r) (res:r) : Type0 =
+unfold let io_post (#r:Type0) (op:io_cmds r) (res:r) : Type0 =
   True
 
-unfold let mio_wps #mst (c:caller) (#r:Type0) (cmd:mio_cmds mst r) : hist #event r =
-  fun (p : hist_post #event r) h ->
-  match cmd with
-  | InEv2 GetTrace ->
+(** Command WP: maps each MIO command to a hist-based WP over io_events. *)
+unfold let mio_cwp #mst (c:caller) (#r:Type0) (op:mio_cmds mst r) : hist #io_event r =
+  fun (p : hist_post #io_event r) h ->
+  match op with
+  | CmdR GetTrace ->
     let p : hist_post (Ghost.erased trace) = p in
     p [] (Ghost.hide h)
-  | InEv2 GetST -> forall (s:mst.typ). s `mst.abstracts` h ==> p [] s
-  | InEv1 iocmd -> io_pre iocmd h /\ (forall (res:r). io_post iocmd res ==> p [convert_call_to_event c iocmd res] res)
+  | CmdR GetST -> forall (s:mst.typ). s `mst.abstracts` h ==> p [] s
+  | CmdL iocmd -> io_pre iocmd h /\ (forall (res:r). io_post iocmd res ==> p [convert_call_to_event c iocmd res] res)
 
 open DMFree
 
-(** Instantiation of the Dijkstra monad from DMFree with MIO events **)
+(** Instantiation of the Dijkstra monad from DMFree with MIO commands/events **)
 
-let mio_dm (mst:mstate) (a:Type) (wp:hist #event a) =
-  dm (mio_cmds mst) event mio_wps a wp
+let mio_dm (mst:mstate) (a:Type) (wp:hist #io_event a) =
+  dm (mio_cmds mst) io_event mio_cwp a wp
 
-let mio_dm_return (mst:mstate) #a (x:a) : mio_dm mst a (hist_return #a #event x) =
-  dm_return event mio_wps x
+let mio_dm_return (mst:mstate) #a (x:a) : mio_dm mst a (hist_return #a #io_event x) =
+  dm_return mio_cwp x
 
 #push-options "--z3rlimit 40"
 let mio_dm_bind (mst:mstate) #a #b
-  (wp_v : hist #event a)
-  (wp_f : a -> hist #event b)
+  (wp_v : hist #io_event a)
+  (wp_f : a -> hist #io_event b)
   (v : mio_dm mst a wp_v)
   (f : (x:a -> mio_dm mst b (wp_f x))) :
   Tot (mio_dm mst b (hist_bind wp_v wp_f)) =
-  dm_bind event mio_wps wp_v wp_f v f
+  dm_bind mio_cwp wp_v wp_f v f
 #pop-options
 
-let mio_dm_subcomp (mst:mstate) #a (wp1 wp2 : hist #event a) (f : mio_dm mst a wp1) :
+let mio_dm_subcomp (mst:mstate) #a (wp1 wp2 : hist #io_event a) (f : mio_dm mst a wp1) :
   Pure (mio_dm mst a wp2)
     (requires wp1 ⊑ wp2)
     (ensures fun _ -> True) =
-  dm_subcomp event mio_wps wp1 wp2 f
+  dm_subcomp mio_cwp wp1 wp2 f
 
 let mio_dm_if_then_else (mst:mstate) #a
-  (wp1 wp2 : hist #event a) (f : mio_dm mst a wp1) (g : mio_dm mst a wp2) (b : bool) : Type =
-  dm_if_then_else event mio_wps wp1 wp2 f g b
+  (wp1 wp2 : hist #io_event a) (f : mio_dm mst a wp1) (g : mio_dm mst a wp2) (b : bool) : Type =
+  dm_if_then_else mio_cwp wp1 wp2 f g b
 
-let mio_dm_partial_return (mst:mstate)
-  (pre:pure_pre) : mio_dm mst (squash pre) (partial_call_wp pre) =
-  dm_partial_return event mio_wps pre
+let mio_dm_guard_return (mst:mstate)
+  (pre:pure_pre) : mio_dm mst (squash pre) (guard_wp pre) =
+  dm_guard_return mio_cwp pre
 
 #push-options "--z3rlimit 40"
 let mio_dm_lift_pure (mst:mstate) #a
   (w : pure_wp a)
   (f : (eqtype_as_type unit -> PURE a w)) :
   mio_dm mst a (wp_lift_pure_hist w) =
-  lift_pure_dm event mio_wps w f
+  lift_pure_dm mio_cwp w f
 #pop-options
